module Data.Vector.Operations where

open import BaseLogic
open import Data.Nat
import Data.Nat.Operations
open import Data.Nat.Relations
open import Data.Nat.Proofs
open import Data.Vector
open import Data.Fin
open import Data.False
open import Data.PropositionalEquality

_^_ : âˆ€ {Î±} (A : Set Î±) (n : Nat) â†’ Set Î±
A ^ n = Vector A n

Vector-first : âˆ€ {Î±} {A : Set Î±} {n : Nat} â†’ Vector A (suc n) â†’ A
Vector-first {Î±} {A} {n} (a âˆ· as) = a

head : âˆ€ {Î±} {A : Set Î±} {n : Nat} â†’ Vector A (suc n) â†’ A
head = Vector-first

Vector-rest : âˆ€ {Î±} {A : Set Î±} {n : Nat} â†’ Vector A (suc n) â†’ Vector A n
Vector-rest {Î±} {A} {n} (a âˆ· as) = as

tail : âˆ€ {Î±} {A : Set Î±} {n : Nat} â†’ Vector A (suc n) â†’ Vector A n
tail = Vector-rest

Vector-coerce-length : âˆ€ {Î±} {A : Set Î±} {m n : Nat} â†’ Vector A m â†’ m â‰¡ n â†’ Vector A n
Vector-coerce-length {Î±} {A} {m} {.m} vec refl = vec

Vector-coerce-type : âˆ€ {Î±} {A B : Set Î±} {n : Nat} â†’ Vector A n â†’ A â‰¡ B â†’ Vector B n
Vector-coerce-type {Î±} {A} {.A} vec refl = vec


_++_ : âˆ€ {Î±} {A : Set Î±} {n m : Nat} â†’ Vector A n â†’ Vector A m â†’ Vector A (Data.Nat.Operations._+_ n m)
[] ++ ys = ys
(x âˆ· xs) ++ ys = x âˆ· (xs ++ ys)

<_> : âˆ€ {Î±} {A : Set Î±} â†’ A â†’ Vector A 1
< x > = (x âˆ· [])

_[_] : âˆ€ {Î±} {A : Set Î±} {n : Nat} â†’ Vector A (suc n) â†’ Fin n â†’ A
(a âˆ· as) [ zero ] =  a
(a âˆ· as) [ suc n ] = as [ n ]

_[_]' : âˆ€ {Î±} {A : Set Î±} {n : Nat} â†’ Vector A n â†’ Fin n â†’ A
(a âˆ· as) [ zero ]' = a
(a âˆ· as) [ suc n ]' = as [ n ]'

lookup : âˆ€ {Î± n} {A : Set Î±} â†’ Fin n â†’ Vector A n â†’ A
lookup zero (x âˆ· xs) = x
lookup (suc i) (x âˆ· xs) = lookup i xs

{-
Note that computationally this is not ideal. In C++ for example, arrays
are strings of bitvectors of a particular length <size>. If we want to
access the element at index i, we use the pointer <array-base> + i*<size>.

We will use these more efficient things, but at another level of abstraction.
-}

data NEVec (A : Set) : Nat â†’ Set where
 end : A â†’ NEVec A (suc zero)
 _âˆ·_ : {n : Nat} â†’ A â†’ NEVec A n â†’ NEVec A (suc n)


get : {A : Set} (n : Nat) â†’ NEVec A (suc n) â†’ (i : Nat) â†’ (i < (suc n)) â†’ A
get {A} zero (end a) zero [ğ•«<ğ•¤ğ•«] = a

-- absurd case: (suc x) â‰® 1
get {A} zero (end a) (suc x) [ğ•¤x<ğ•¤ğ•«] = Ï‰ â˜¢
 where
--proof that this is a throwaway case:
  â˜¢ : âŠ¥
  â˜¢ = ğ•¤xâ‰®1 x [ğ•¤x<ğ•¤ğ•«]

{-
Agda doesn't know there's a conflict between zero and (a âˆ· as) here

We can operate on the knowledge that this is actually an impossible case
and just return a throwaway value `a`.

Prove that these are throwaways by proving that the assumptions lead to contradiction
and using the âŠ¥-elim
-}
-- absurd case: no (a âˆ· as) of length 1
get {A} zero (a âˆ· as) zero [ğ•«<ğ•¤ğ•«] = a
{-
 where
  â˜¢ : âŠ¥

-- Not sure how to prove that NEVec Nat (suc zero) cannot have the form (a âˆ· as)
-- Maybe if we can prove that as : NEVec Nat zero and NEVec Nat zero â†’ âŠ¥

-}  

-- absurd case: no (a âˆ· as) of length 1, and (suc x) â‰® 1
get {A} zero (a âˆ· as) (suc x) [ğ•¤x<ğ•¤ğ•«] = Ï‰ â˜¢
 where
  â˜¢ : âŠ¥
  â˜¢ = ğ•¤xâ‰®1 x [ğ•¤x<ğ•¤ğ•«]

{-
Agda knows there's a conflict between (suc n) and (end a) here

-- absurd case: no (end a) of length > 1
get {A} (suc n) (end a) zero [ğ•«<ğ•¤ğ•¤n] = a

-- absurd case: no (end a) of length > 1
get {A} (suc n) (end a) (suc x) [ğ•¤x<ğ•¤ğ•¤n] = a
-}

get {A} (suc n) (a âˆ· as) zero [ğ•«<ğ•¤ğ•¤n] = a
get {A} (suc n) (a âˆ· as) (suc x) [ğ•¤x<ğ•¤ğ•¤n] = get {A} n as x [x<ğ•¤n]
 where
  [x<ğ•¤n] : x < suc n
  [x<ğ•¤n] = [ğ•¤x<ğ•¤y]â†’[x<y] x (suc n) [ğ•¤x<ğ•¤ğ•¤n]




data NEVecâ‚‚ (A : Set) : (n : Nat) â†’ n > 0 â†’ Set where
 end : A â†’ NEVecâ‚‚ A 1 1>0 
 _âˆ·_ : {n : Nat} {[n>0] : n > 0} â†’ A â†’ NEVecâ‚‚ A n [n>0] â†’ NEVecâ‚‚ A (suc n) ([x>0]â†’[ğ•¤x>0] n [n>0])

-- x [ i ]:= y ...
-- replace the value at index i in vector x with the value y
_[_]:=_ : âˆ€ {Î±} {A : Set Î±} {n : Nat} â†’ Vector A (suc n) â†’ Fin n â†’ A â†’ Vector A (suc n)
(x âˆ· xs) [ zero ]:= y = y âˆ· xs
(x âˆ· xs) [ suc i ]:= y = x âˆ· (xs [ i ]:= y)
